| Basis | x_0 | x_1 | x_2 |
| ----- | --- | --- | --- |
| s_0   | 0   | 1   | 1   |
| s_1   | 0   | -1  | -2  |
| s_2   | 3   | -3  | 2   |
| s_3   | -2  | 0   | 1   |
| s_4   | 3   | 2   | 1   |

| Basis   | s_4[-3] | x_1[0] | x_2[0] |
| ------- | ------- | ------ | ------ |
| s_0[0]  | 0       | 1      | 1      |
| s_1[0]  | 0       | -1     | -2     |
| s_2[-3] | 1       | -5     | 1      |
| s_3[2]  | -2/3    | 4/3    | 4/3    |
| x_0[-1] | 1/3     | -2/3   | -1/3   |

| Basis     | s_4[-3] | s_0[-2] | x_2[0] |
| --------- | ------- | ------- | ------ |
| x_1[-2]   | 0       | 1       | -1     |
| s_1[2]    | 0       | -1      | -1     |
| s_2[7]    | 1       | -5      | 6      |
| s_3[-2/3] | -2/3    | 4/3     | 0      |
| x_0[1/3]  | 1/3     | -2/3    | 1/3    |



**x_1 = s_0 - x_2 **

s_1 = -1(s_0 - x_2) -2x_2 
s_1 = -s_0 +x_2 -2x_2
s_1 = -s_0 -x_2

s_2 = s_4 -5(s_0 - x_2) +x_2
s_2 = s_4 -5s_0 +5x_2 +x_2 
s_2 = s_4 -5s_0 +6s_2

s_3 = -2/3s_4 +4/3(s_0 - x_2) +4/3x_2
s_3 = -2/3s_4 +4/3s_0 

x_0 = 1/3s_4 -2/3(s_0 - x_2) -1/3x_2
x_0 = 1/3s_4 -2/3s_0 + 2/3x_2 -1/3x_2
x_0 = 1/3s_4 -2/3s_0  +1/3x_2
