$\varphi_{1} := \forall x\Bigl( (\exists y(S(x,y)\lor T(x,y))) \to (\exists y \forall x (P(x) \to (S(y,x)\land S(x,c))))\Bigr)$

$\forall x\Bigl( (\exists y(S(x,y)\lor T(x,y))) \to (\exists y \forall x (\neg P(x) \lor (S(y,x)\land S(x,c))))\Bigr)$

$\forall x\Bigl( \neg(\exists y(S(x,y)\lor T(x,y))) \lor (\exists y \forall x (\neg P(x) \lor (S(y,x)\land S(x,c))))\Bigr)$

$\forall x\Bigl(\forall y(\neg S(x,y)\land \neg T(x,y)) \lor (\exists y \forall x (\neg P(x) \lor (S(y,x)\land S(x,c))))\Bigr)$

Die Formel ist nun in NNF jetzt können wir sie in Pränex-Normalform umwandeln:

$\forall x\Bigl(\forall y(\neg S(x,y)\land \neg T(x,y)) \lor (\exists y \forall x (\neg P(x) \lor (S(y,x)\land S(x,c))))\Bigr)$

Gebundene Umbenennung:

$\forall x\Bigl(\forall y(\neg S(x,y)\land \neg T(x,y)) \lor (\exists w \forall z (\neg P(z) \lor (S(w,z)\land S(z,c))))\Bigr)$